### Question 15

Give the values of i and j after each of the following expression statements has been executed. (Assume that i has the value 1 initially and j has the value 2.)  
(a) i += j;  
(b) i--;  
(c) i * j / i;  
(d) i % ++j;

### Solution

(a)  
i += j  
i = i + j  
i = 1 + 2  
i = 3

j = 2

(b)  
i--  
i = 0  

j = 2

(c)  
i * j / i  
(1 * 2) / 1  
2 / 1  
2

i = 1  
j = 2  
Since the expression does not have a side effect the original values of i and j remains unchanged.

(d)  
i % ++j  
1 % 3  
1

i = 1  
j = 3
